Fix proofs about compute_console

progs/io_os_connection.v
@@ -7,6 +7,7 @@ Require Import compcert.lib.Integers.
 Require Import compcert.common.Memory.
 Require Import VST.progs.io_specs.
 Require Import VST.progs.io_dry.
+Require Import VST.progs.io_os_specs.
 Require Import VST.floyd.sublist.
 Import ExtLib.Structures.Monad.
 
@@ -14,6 +15,14 @@ Local Ltac inj :=
   repeat match goal with
   | H: _ = _ |- _ => assert_succeeds (injection H); inv H
   end.
+
+Ltac simpl_rev :=
+  repeat (rewrite rev_app_distr; cbn [rev app]);
+  rewrite <- ?app_assoc; cbn [rev app].
+
+Ltac simpl_rev_in H :=
+  repeat (rewrite rev_app_distr in H; cbn [rev app] in H);
+  rewrite <- ?app_assoc in H; cbn [rev app] in H.
 
 (** Helper Lemmas *)
 Section ListFacts.
@@ -228,37 +237,31 @@ Definition getchar_post' (m0 m : mem) r (witness : (int -> IO_itree) * IO_itree)
     let (_, z0) := witness in z = z0 /\ Int.signed r = -1).
 
 (** Traces *)
-Inductive IO_trace_event :=
-| ETReadOS (ridx : nat) (r : Z)
-| ETReadUser (ridx : nat) (r : Z)
-| ETWrite (c : Z).
-Definition etrace := list IO_trace_event.
+Definition ostrace := list IOEvent.
 
-Definition IO_trace_event_eq (e1 e2 : IO_trace_event) : {e1 = e2} + {e1 <> e2} :=
+Definition IOEvent_eq (e1 e2 : IOEvent) : {e1 = e2} + {e1 <> e2} :=
   ltac:(repeat decide equality).
 
-Definition trace_event_rtype (e : IO_trace_event) :=
+Definition trace_event_rtype (e : IOEvent) :=
   match e with
-  | ETReadOS _ _ => void
-  | ETReadUser _ _ => int
-  | ETWrite _ => unit
+  | IOEvRecv _ _ _ => void
+  | IOEvGetc _ _ _ => int
   end.
 
-Definition io_event_of_io_tevent (e : IO_trace_event)
+Definition io_event_of_io_tevent (e : IOEvent)
   : option (IO_event (trace_event_rtype e) * (trace_event_rtype e)) :=
   match e with
-  | ETReadOS _ _ => None
-  | ETReadUser _ r => Some (ERead, Int.repr r)
-  | ETWrite c => Some (EWrite (Int.repr c), tt)
+  | IOEvRecv _ _ _ => None
+  | IOEvGetc _ _ r => Some (ERead, Int.repr r)
   end.
 
-Fixpoint trace_of_etrace (t : etrace) : @trace IO_event unit :=
+Fixpoint trace_of_ostrace (t : ostrace) : @trace IO_event unit :=
   match t with
   | nil => TEnd
   | e :: t' =>
       match io_event_of_io_tevent e with
-      | Some (e', r) => TEventResponse e' r (trace_of_etrace t')
-      | _ => trace_of_etrace t'
+      | Some (e', r) => TEventResponse e' r (trace_of_ostrace t')
+      | _ => trace_of_ostrace t'
       end
   end.
 
@@ -284,188 +287,176 @@ Section SanityChecks.
     repeat constructor.
   Qed.
 
-  Goal is_trace tree (trace_of_etrace nil).
+  Goal is_trace tree (trace_of_ostrace nil).
   Proof.
     hnf; cbn.
     constructor.
   Qed.
 
-  Goal is_trace tree (trace_of_etrace (ETReadUser O 0 :: ETReadOS O 0 :: nil)).
+  Goal is_trace tree (trace_of_ostrace (IOEvGetc 0 O 0 :: IOEvRecv 0 O 0 :: nil)).
   Proof.
     hnf; cbn.
     repeat constructor.
   Qed.
 End SanityChecks.
 
-(** CertiKOS Specs *)
-Section Specs.
-
-  Class ConsoleLen := {
-    CONSOLE_MAX_LEN : Z;
-    console_len_pos : 0 < CONSOLE_MAX_LEN
-  }.
-  Context `{ConsoleLen}.
-
-  Class SerialOracle := {
-    serial_oracle : etrace -> Z;
-    serial_oracle_in_range : forall tr,
-      0 <= serial_oracle tr <= 255
-  }.
-  Context `{SerialOracle}.
-
-  Record state := mkSt {
-    st_mem : mem;
-    st_trace : etrace;
-  }.
-
-  Fixpoint compute_console (tr : etrace) : list (Z * nat) :=
-    match tr with
-    | nil => nil
-    | ev :: tr' =>
-        let cons := compute_console tr' in
-        match ev with
-        | ETReadOS ridx c =>
-            let cons' := if Zlength cons <? CONSOLE_MAX_LEN then cons
-                         else tl cons in
-            cons' ++ (c, ridx) :: nil
-        | ETReadUser _ _ => tl cons
-        | _ => cons
-        end
-    end.
-
-  (* Read a character from the serial device and place it in the console buffer.
-     Triggered by an interrupt from the serial device. *)
-  Definition serial_getc (st : state) : state :=
-    let (mem, tr) := st in
-    let c := serial_oracle tr in
-    let ridx := length tr in
-    mkSt mem (ETReadOS ridx c :: tr).
-
-  (* Take the first element from the console buffer or -1 if it is empty. *)
-  Definition console_read (st : state) : state * Z :=
-    let (mem, tr) := st in
-    match compute_console tr with
-    | nil => (st, -1)
-    | (c, ridx) :: _ =>
-      let st' := mkSt mem (ETReadUser ridx c :: tr) in
-      (st', c)
-    end.
-
-  (* Return the new state, the read character, and the section of the trace to
-     be consumed. *)
-  Definition getchar_spec (st : state) : state * Z :=
-    let (st', r) := console_read st in
-    (* Success *)
-    if 0 <=? r then (st', r)
-    (* Error *)
-    else (st', -1).
-
-End Specs.
-
 (** Trace Invariants *)
 Section Invariants.
 
-  Context {Hclen : ConsoleLen} {Horacle : SerialOracle}.
+  Fixpoint compute_console' (tr : ostrace) : list (Z * Z * nat) :=
+    match tr with
+    | nil => nil
+    | ev :: tr' =>
+      let cons := compute_console' tr' in
+      match ev with
+      | IOEvRecv logIdx strIdx c =>
+        let cons' := if Zlength cons <? CONS_BUFFER_MAX_CHARS then cons else tl cons in
+        cons' ++ (c, logIdx, strIdx) :: nil
+      | IOEvGetc _ _ _ => tl cons
+      end
+    end.
+  Definition compute_console tr := compute_console' (rev tr).
+
+  Lemma app_tail_case' {A} : forall (xs ys ys' : list A) x,
+    xs ++ x :: nil = ys ++ ys' ->
+    ys' = nil \/
+    exists ys'', xs = ys ++ ys'' /\ ys' = ys'' ++ x :: nil.
+  Proof.
+    intros * Heq.
+    assert (Hcase: ys' = nil \/ exists ys'' y'', ys' = ys'' ++ y'' :: nil).
+    { clear; induction ys'; auto.
+      intuition (subst; eauto using app_nil_l).
+      destruct H as (? & ? & ?); subst.
+      eauto using app_comm_cons.
+    }
+    destruct Hcase as [? | (? & ? & ?)]; subst; auto.
+    rewrite app_assoc in Heq.
+    apply app_inj_tail in Heq.
+    intuition (subst; eauto).
+  Qed.
 
   (* Everything in the trace was put there by the serial device. *)
   Definition valid_trace_serial tr :=
-    forall ridx c pre post,
-      tr = post ++ ETReadOS ridx c :: pre ->
-      serial_oracle pre = c /\ length pre = ridx.
+    forall logIdx strIdx c pre post,
+      tr = pre ++ IOEvRecv logIdx strIdx c :: post ->
+      Zlength pre = logIdx + Z.of_nat strIdx /\
+      match SerialEnv logIdx with
+      | SerialRecv str => nth_error str strIdx = Some c
+      | _ => False
+      end.
 
   (* Every user read has a matching OS read earlier in the trace. *)
   Definition valid_trace_user tr :=
-    forall ridx c pre post,
-      tr = post ++ ETReadUser ridx c :: pre ->
-      In (ETReadOS ridx c) pre /\ hd_error (compute_console pre) = Some (c, ridx).
+    forall logIdx strIdx c pre post,
+      tr = pre ++ IOEvGetc logIdx strIdx c :: post ->
+      In (IOEvRecv logIdx strIdx c) pre /\ hd_error (compute_console pre) = Some (c, logIdx, strIdx).
 
   (* Every event in the trace is unique. *)
-  Definition valid_trace_unique (tr : etrace) := NoDup tr.
+  Definition valid_trace_unique (tr : ostrace) := NoDup tr.
 
   (* All trace invariants hold. *)
-  Record valid_trace st := {
-    vt_trace_serial : valid_trace_serial st.(st_trace);
-    vt_trace_user : valid_trace_user st.(st_trace);
-    vt_trace_unique : valid_trace_unique st.(st_trace);
+  Record valid_trace (st : RData) := {
+    vt_trace_serial : valid_trace_serial st.(io_log);
+    vt_trace_user : valid_trace_user st.(io_log);
+    vt_trace_unique : valid_trace_unique st.(io_log);
   }.
 
   (* Compute the newly added events in the trace. *)
-  Definition new_trace (st st' : state) : etrace :=
-    fst (split_at_common_suffix IO_trace_event_eq st.(st_trace) st'.(st_trace)).
+  (* Definition new_trace (st st' : state) : ostrace := *)
+  (*   fst (split_at_common_suffix IO_trace_event_eq st.(io_log) st'.(io_log)). *)
 
   (* Invariants about the returned character and traces. *)
-  Definition valid_ret (st st' : state) (c : Z) :=
-    (* c is in the proper range. *)
-    (c = -1 \/ 0 <= c <= 255) /\
-    (* The memory is unchanged. *)
-    st.(st_mem) = st'.(st_mem) /\
-    let t := new_trace st st' in
-    (* The new trace is the old one plus the newly added events. *)
-    st'.(st_trace) = t ++ st.(st_trace) /\
-    (* The newly added events are either nil or a single user read. *)
-    (c = -1 -> t = nil) /\
-    (0 <= c <= 255 -> exists ridx, t = ETReadUser ridx c :: nil).
+  (* Definition valid_ret (st st' : state) (c : Z) := *)
+  (*   (1* c is in the proper range. *1) *)
+  (*   (c = -1 \/ 0 <= c <= 255) /\ *)
+  (*   (1* The memory is unchanged. *1) *)
+  (*   st.(st_mem) = st'.(st_mem) /\ *)
+  (*   let t := new_trace st st' in *)
+  (*   (1* The new trace is the old one plus the newly added events. *1) *)
+  (*   st'.(io_log) = t ++ st.(io_log) /\ *)
+  (*   (1* The newly added events are either nil or a single user read. *1) *)
+  (*   (c = -1 -> t = nil) /\ *)
+  (*   (0 <= c <= 255 -> exists logIdx, t = IOEvGetc logIdx c :: nil). *)
 
-  Lemma valid_trace_serial_cons : forall tr ev,
-    valid_trace_serial (ev :: tr) ->
+  Lemma valid_trace_serial_snoc : forall tr ev,
+    valid_trace_serial (tr ++ ev :: nil) ->
     valid_trace_serial tr.
   Proof.
     unfold valid_trace_serial.
-    intros; subst; eauto using app_comm_cons.
+    intros * Hvalid * ->; eapply Hvalid.
+    rewrite app_comm_cons, <- app_assoc; eauto.
   Qed.
+
+  Lemma cons_app_single {A} : forall (xs ys : list A) x,
+    xs ++ x :: ys = (xs ++ x :: nil) ++ ys.
+  Proof. intros; rewrite <- app_assoc; auto. Qed.
 
   Lemma valid_trace_serial_app : forall tr' tr,
-    valid_trace_serial (tr' ++ tr) ->
+    valid_trace_serial (tr ++ tr') ->
     valid_trace_serial tr.
   Proof.
-    induction tr'; cbn; eauto using valid_trace_serial_cons.
+    induction tr'; cbn; intros *.
+    - rewrite app_nil_r; auto.
+    - rewrite cons_app_single.
+      eauto using valid_trace_serial_snoc.
   Qed.
 
-  Local Hint Resolve valid_trace_serial_cons valid_trace_serial_app.
+  Local Hint Resolve valid_trace_serial_snoc valid_trace_serial_app.
 
-  Lemma read_os_ordered : forall mid pre ridx c ridx' c',
-    valid_trace_serial (ETReadOS ridx' c' :: mid ++ ETReadOS ridx c :: pre) ->
-    (ridx < ridx')%nat.
+  Lemma read_os_ordered : forall post mid pre logIdx strIdx c logIdx' strIdx' c',
+    valid_trace_serial (pre ++ IOEvRecv logIdx strIdx c :: mid ++ IOEvRecv logIdx' strIdx' c' :: post) ->
+    logIdx + Z.of_nat strIdx < logIdx' + Z.of_nat strIdx'.
   Proof.
     intros * Hvalid.
-    edestruct (Hvalid ridx); eauto using app_comm_cons.
-    edestruct (Hvalid ridx'); eauto using app_nil_l.
-    subst; rewrite app_length; cbn; lia.
+    edestruct (Hvalid logIdx) as (Hlen & ?); eauto; intros.
+    edestruct (Hvalid logIdx') as (Hlen' & ?); intros.
+    { rewrite app_comm_cons, app_assoc; eauto. }
+    pose proof (Zlength_nonneg mid).
+    rewrite Zlength_app, Zlength_cons in Hlen'.
+    lia.
   Qed.
 
-  Lemma in_console_in_trace : forall tr ridx c,
-    In (c, ridx) (compute_console tr) ->
-    In (ETReadOS ridx c) tr.
+  Lemma in_console_in_trace' : forall tr logIdx strIdx c,
+    In (c, logIdx, strIdx) (compute_console' tr) ->
+    In (IOEvRecv logIdx strIdx c) tr.
   Proof.
-    induction tr as [| ev tr]; cbn; intros * Hin; auto.
-    destruct ev; cbn in Hin; auto using in_tail.
+    induction tr as [| ev tr]; cbn; intros * Hin; eauto.
+    destruct ev; auto using in_tail.
     rewrite in_app_iff in Hin; cbn in Hin.
-    intuition (inj; auto).
+    intuition (inj; auto); right.
     destruct (_ <? _); auto using in_tail.
   Qed.
 
-  Lemma console_trace_same_order : forall tr pre mid post ridx c ridx' c',
-    compute_console tr = pre ++ (c, ridx) :: mid ++ (c', ridx') :: post ->
+  Corollary in_console_in_trace : forall tr logIdx strIdx c,
+    In (c, logIdx, strIdx) (compute_console tr) ->
+    In (IOEvRecv logIdx strIdx c) tr.
+  Proof.
+    unfold compute_console; intros * Hin.
+    apply in_rev.
+    apply in_console_in_trace'; auto.
+  Qed.
+
+  Lemma console_trace_same_order' : forall tr pre mid post logIdx strIdx c logIdx' strIdx' c',
+    compute_console' tr = pre ++ (c, logIdx, strIdx) :: mid ++ (c', logIdx', strIdx') :: post ->
     exists pre' mid' post',
-      tr = post' ++ ETReadOS ridx' c' :: mid' ++ ETReadOS ridx c :: pre'.
+      tr = post' ++ IOEvRecv logIdx' strIdx' c' :: mid' ++ IOEvRecv logIdx strIdx c :: pre'.
   Proof.
     induction tr as [| ev tr]; cbn; intros * Hcons;
       [contradict Hcons; auto using app_cons_not_nil |].
-    destruct ev; cbn in Hcons;
-      try solve [edestruct IHtr as (? & ? & ? & ?); eauto; subst; eauto using app_comm_cons].
+    destruct ev; cbn in Hcons.
     - rewrite app_comm_cons, app_assoc in Hcons.
       destruct @app_tail_case with (1 := Hcons) as [(? & ? & Hcons') | (? & Hcons' & ?)]; inj; subst;
         destruct (_ <? _).
-      + assert (Hin: In (c, ridx) (compute_console tr)).
+      + assert (Hin: In (c, logIdx, strIdx) (compute_console' tr)).
         { rewrite Hcons', in_app_iff; cbn; auto. }
-        apply in_console_in_trace in Hin.
+        apply in_console_in_trace' in Hin.
         apply in_split in Hin; destruct Hin as (? & ? & ?); subst; eauto using app_nil_l.
       + apply tail_not_nil_has_head in Hcons'; auto using app_cons_not_nil.
         destruct Hcons' as (? & Hcons').
         rewrite app_comm_cons in Hcons'.
-        assert (Hin: In (c, ridx) (compute_console tr)).
+        assert (Hin: In (c, logIdx, strIdx) (compute_console' tr)).
         { rewrite Hcons', in_app_iff; cbn; auto. }
-        apply in_console_in_trace in Hin.
+        apply in_console_in_trace' in Hin.
         apply in_split in Hin; destruct Hin as (? & ? & Heq); subst; eauto using app_nil_l.
       + rewrite <- app_assoc, <- app_comm_cons in Hcons'.
         edestruct IHtr as (? & ? & ? & Heq'); eauto; subst; eauto using app_comm_cons.
@@ -475,8 +466,8 @@ Section Invariants.
         rewrite app_comm_cons in Hcons'.
         edestruct IHtr as (? & ? & ? & Heq); eauto; subst; eauto using app_comm_cons.
     - assert (Hcons': exists el,
-        compute_console tr = el :: pre ++ (c, ridx) :: mid ++ (c', ridx') :: post).
-      { destruct (compute_console tr); cbn in Hcons; subst; eauto.
+        compute_console' tr = el :: pre ++ (c, logIdx, strIdx) :: mid ++ (c', logIdx', strIdx') :: post).
+      { destruct (compute_console' tr); cbn in Hcons; subst; eauto.
         contradict Hcons; auto using app_cons_not_nil.
       }
       destruct Hcons' as (? & Hcons').
@@ -484,89 +475,107 @@ Section Invariants.
         edestruct IHtr as (? & ? & ? & Heq); eauto; subst; eauto using app_comm_cons.
   Qed.
 
-  Corollary console_tl_trace_same_order : forall tr ridx c ridx' c',
-    hd_error (compute_console tr) = Some (c, ridx) ->
-    hd_error (tl (compute_console tr)) = Some (c', ridx') ->
+  Corollary console_tl_trace_same_order' : forall tr logIdx strIdx c logIdx' strIdx' c',
+    hd_error (compute_console' tr) = Some (c, logIdx, strIdx) ->
+    hd_error (tl (compute_console' tr)) = Some (c', logIdx', strIdx') ->
     exists pre' mid' post',
-      tr = post' ++ ETReadOS ridx' c' :: mid' ++ ETReadOS ridx c :: pre'.
+      tr = post' ++ IOEvRecv logIdx' strIdx' c' :: mid' ++ IOEvRecv logIdx strIdx c :: pre'.
   Proof.
     intros * Hcons Hcons'.
-    destruct (compute_console tr) as [| ? cons] eqn:Heq; cbn in Hcons, Hcons'; [easy |]; inj.
+    destruct (compute_console' tr) as [| ? cons] eqn:Heq; cbn in Hcons, Hcons'; [easy |]; inj.
     destruct cons as [| ? cons'] eqn:Heq'; cbn in Hcons'; [easy |]; inj.
-    eapply console_trace_same_order.
+    eapply console_trace_same_order'.
     instantiate (1 := cons'); repeat instantiate (1 := nil); eauto.
   Qed.
 
-  Lemma compute_console_ordered : forall tr ev ridx c ridx' c',
-    let cons := compute_console tr in
-    let cons' := compute_console (ev :: tr) in
-    valid_trace_serial (ev :: tr) ->
-    hd_error cons = Some (c, ridx) ->
-    hd_error cons' = Some (c', ridx') ->
+  Lemma compute_console_ordered' : forall tr ev logIdx strIdx c logIdx' strIdx' c',
+    let cons := compute_console' tr in
+    let cons' := compute_console' (ev :: tr) in
+    valid_trace_serial (rev tr ++ ev :: nil) ->
+    hd_error cons = Some (c, logIdx, strIdx) ->
+    hd_error cons' = Some (c', logIdx', strIdx') ->
     match ev with
-    | ETReadUser _ _ => (ridx < ridx')%nat
-    | _ => (ridx <= ridx')%nat
+    | IOEvGetc _ _ _ => logIdx + Z.of_nat strIdx < logIdx' + Z.of_nat strIdx'
+    | _ => logIdx + Z.of_nat strIdx <= logIdx' + Z.of_nat strIdx'
     end.
   Proof.
     intros * Hserial Hcons Hcons'; subst cons cons'.
     destruct ev; cbn in Hcons'.
     - destruct (_ <? _).
-      + erewrite hd_error_app in Hcons'; eauto; inj; auto.
-      + destruct (hd_error_app_case (tl (compute_console tr)) (r, ridx0)) as [Heq | Heq];
+      + erewrite hd_error_app in Hcons'; eauto; inj; lia.
+      + destruct (hd_error_app_case (tl (compute_console' tr)) (c0, logIdx0, strIdx0)) as [Heq | Heq];
           rewrite Heq in Hcons'; clear Heq.
-        * edestruct console_tl_trace_same_order as (? & ? & ? & Heq); eauto; subst.
-          rewrite app_comm_cons in Hserial.
-          apply valid_trace_serial_app in Hserial.
-          eapply read_os_ordered in Hserial; eauto; lia.
+        * edestruct console_tl_trace_same_order' as (? & ? & ? & Heq); eauto; subst.
+          simpl_rev_in Hserial.
+          eapply read_os_ordered in Hserial; lia.
         * cbn in Hcons'; inj.
           apply hd_error_in in Hcons.
-          apply in_console_in_trace in Hcons.
+          apply in_console_in_trace' in Hcons.
           apply in_split in Hcons; destruct Hcons as (? & ? & ?); subst.
+          simpl_rev_in Hserial.
           apply read_os_ordered in Hserial; lia.
-    - edestruct console_tl_trace_same_order as (? & ? & ? & Heq); eauto; subst.
+    - edestruct console_tl_trace_same_order' as (? & ? & ? & Heq); eauto; subst.
+      simpl_rev_in Hserial.
       eapply read_os_ordered; eauto.
-    - rewrite Hcons in Hcons'; inj; auto.
   Qed.
 
-  Lemma compute_console_user_ridx_increase : forall post pre ridx c ridx' c',
-    let tr := post ++ ETReadUser ridx c :: pre in
-    let cons := compute_console pre in
-    let cons' := compute_console tr in
-    valid_trace_serial tr ->
-    hd_error cons = Some (c, ridx) ->
-    hd_error cons' = Some (c', ridx') ->
-    (ridx < ridx')%nat.
+  Lemma compute_console_user_idx_increase' : forall post pre logIdx strIdx c logIdx' strIdx' c',
+    let tr := post ++ IOEvGetc logIdx strIdx c :: pre in
+    let cons := compute_console' pre in
+    let cons' := compute_console' tr in
+    valid_trace_serial (rev tr) ->
+    hd_error cons = Some (c, logIdx, strIdx) ->
+    hd_error cons' = Some (c', logIdx', strIdx') ->
+    logIdx + Z.of_nat strIdx < logIdx' + Z.of_nat strIdx'.
   Proof.
-    induction post as [| ev post]; intros * Hserial Hcons Hcons'; subst tr cons cons'.
-    - eapply compute_console_ordered in Hcons; eauto.
-      cbn in Hcons; auto.
+    induction post as [| ev post]; intros * Hserial Hcons Hcons'; subst tr cons cons'; simpl_rev_in Hserial.
+    - eapply compute_console_ordered' in Hcons; eauto.
+      cbn in Hcons, Hcons'; auto.
     - assert (Hcase:
-        (exists ridx'' c'',
-          hd_error (compute_console (post ++ ETReadUser ridx c :: pre)) = Some (c'', ridx'')) \/
-        ev = ETReadOS ridx' c' /\ compute_console (post ++ ETReadUser ridx c :: pre) = nil).
+        (exists logIdx'' strIdx'' c'',
+          hd_error (compute_console' (post ++ IOEvGetc logIdx strIdx c :: pre)) = Some (c'', logIdx'', strIdx'')) \/
+        ev = IOEvRecv logIdx' strIdx' c' /\ compute_console' (post ++ IOEvGetc logIdx strIdx c :: pre) = nil).
       { cbn in Hcons'; destruct ev; eauto.
-        - destruct (compute_console (post ++ _ :: pre)) as [| (? & ?) ?] eqn:?; cbn; eauto.
+        - destruct (compute_console' (post ++ _ :: pre)) as [| ((? & ?) & ?) ?] eqn:?; cbn; eauto.
           right; destruct (_ <? _); cbn in Hcons'; inj; eauto.
         - eapply hd_error_tl in Hcons'.
-          destruct Hcons' as ((? & ?) & ?); eauto.
+          destruct Hcons' as (((? & ?) & ?) & ?); eauto.
       }
-      destruct Hcase as [(ridx'' & c'' & Hcons'') | (? & Hcons'')]; subst.
-      + enough (ridx < ridx'' <= ridx')%nat by lia.
-        split; eauto.
-        destruct ev; eapply compute_console_ordered in Hcons'; eauto; lia.
+      destruct Hcase as [(logIdx'' & strIdx'' & c'' & Hcons'') | (? & Hcons'')]; subst.
+      + enough (logIdx + Z.of_nat strIdx < logIdx'' + Z.of_nat strIdx'' <= logIdx' + Z.of_nat strIdx') by lia.
+        split.
+        * eapply IHpost with (pre := pre); simpl_rev; eauto.
+          eapply valid_trace_serial_snoc.
+          rewrite <- app_assoc, <- app_comm_cons; eauto.
+        * rewrite <- app_comm_cons in Hcons'.
+          eapply compute_console_ordered' in Hcons'; eauto; simpl_rev; eauto.
+          destruct ev; lia.
       + apply hd_error_in in Hcons.
-        apply in_console_in_trace in Hcons.
+        apply in_console_in_trace' in Hcons.
         apply in_split in Hcons; destruct Hcons as (? & ? & ?); subst.
-        rewrite <- app_comm_cons in Hserial.
-        rewrite (app_comm_cons _ _ (ETReadUser _ _)) in Hserial.
+        simpl_rev_in Hserial.
+        rewrite (app_comm_cons _ _ (IOEvGetc _ _ _)) in Hserial.
         rewrite app_assoc in Hserial.
         eauto using read_os_ordered.
   Qed.
 
-  Lemma console_len : forall tr,
-    Zlength (compute_console tr) <= CONSOLE_MAX_LEN.
+  Corollary compute_console_user_idx_increase : forall pre post logIdx strIdx c logIdx' strIdx' c',
+    let tr := pre ++ IOEvGetc logIdx strIdx c :: post in
+    let cons := compute_console pre in
+    let cons' := compute_console tr in
+    valid_trace_serial tr ->
+    hd_error cons = Some (c, logIdx, strIdx) ->
+    hd_error cons' = Some (c', logIdx', strIdx') ->
+    logIdx + Z.of_nat strIdx < logIdx' + Z.of_nat strIdx'.
   Proof.
-    pose proof console_len_pos.
+    unfold compute_console; intros *; simpl_rev; intros Hserial Hcons Hcons'.
+    eapply compute_console_user_idx_increase'; eauto.
+    simpl_rev; rewrite !rev_involutive; auto.
+  Qed.
+
+  Lemma console_len' : forall tr,
+    Zlength (compute_console' tr) <= CONS_BUFFER_MAX_CHARS.
+  Proof.
     induction tr as [| ev tr]; cbn; try lia.
     destruct ev; cbn; auto.
     - destruct (_ <? _) eqn:Hlt; [rewrite Z.ltb_lt in Hlt | rewrite Z.ltb_nlt in Hlt];
@@ -575,6 +584,10 @@ Section Invariants.
       intros Hcons; rewrite Hcons in *; cbn in *; lia.
     - etransitivity; [apply Zlength_tail |]; auto.
   Qed.
+
+  Corollary console_len : forall tr,
+    Zlength (compute_console tr) <= CONS_BUFFER_MAX_CHARS.
+  Proof. intros; apply console_len'. Qed.
 
   (** Trace Invariants Preserved *)
   Lemma serial_getc_preserve_valid_trace : forall st st',
@@ -607,7 +620,7 @@ Section Invariants.
   Proof.
     unfold console_read; intros * Hvalid Hspec.
     destruct st as [? tr]; destruct Hvalid; cbn in *.
-    destruct (compute_console tr) as [| (c' & ridx) cons] eqn:Hcons; inj.
+    destruct (compute_console tr) as [| (c' & logIdx & strIdx) cons] eqn:Hcons; inj.
     - repeat (split; auto).
     - split; cbn; red; auto using in_tail.
       + (* valid_trace_serial *)
@@ -616,7 +629,7 @@ Section Invariants.
       + (* valid_trace_user *)
         intros * Heq.
         symmetry in Heq; destruct post; inj; cbn in *; eauto.
-        assert (Hin: In (ETReadOS ridx c) tr).
+        assert (Hin: In (IOEvRecv logIdx strIdx c) tr).
         { apply in_console_in_trace.
           rewrite Hcons; cbn; auto.
         }
@@ -629,8 +642,8 @@ Section Invariants.
         apply in_split in Hin.
         destruct Hin as (post & pre & ?); subst.
         edestruct vt_trace_user0 as (Hin & Hhd); eauto.
-        enough (ridx < ridx)%nat by lia.
-        eapply compute_console_user_ridx_increase; eauto.
+        enough logIdx + strIdx < logIdx + strIdx by lia.
+        eapply compute_console_user_idx_increase; eauto.
         rewrite Hcons; cbn; auto.
   Qed.
 
@@ -653,12 +666,12 @@ Section Invariants.
   Proof.
     unfold console_read; intros * Hvalid Hspec.
     destruct st as [? tr]; destruct Hvalid; cbn in *.
-    destruct (compute_console tr) as [| (c' & ridx) cons] eqn:Hcons; inj.
+    destruct (compute_console tr) as [| (c' & logIdx & strIdx) cons] eqn:Hcons; inj.
     - repeat (split; eauto using common_suffix_full); cbn -[common_suffix]; try lia.
       all: rewrite Nat.leb_refl, common_suffix_full, Nat.sub_diag; cbn; auto.
     - repeat split.
       + (* c in range *)
-        assert (Hin: In (ETReadOS ridx c) tr).
+        assert (Hin: In (IOEvRecv logIdx strIdx c) tr).
         { apply in_console_in_trace.
           rewrite Hcons; cbn; auto.
         }
@@ -673,7 +686,7 @@ Section Invariants.
         { cbn; eauto. }
         clear; induction tr; auto.
       + (* empty trace *)
-        assert (Hin: In (ETReadOS ridx c) tr).
+        assert (Hin: In (IOEvRecv logIdx strIdx c) tr).
         { apply in_console_in_trace.
           rewrite Hcons; cbn; auto.
         }
@@ -712,8 +725,8 @@ Section SpecsCorrect.
   (* For any trace that the new itree (z) allows, the old itree (z0) allowed it
      with the generated trace (t) as a prefix. *)
 
-  Definition consume_trace (z0 z : IO_itree) (et : etrace) :=
-    let t := trace_of_etrace et in
+  Definition consume_trace (z0 z : IO_itree) (et : ostrace) :=
+    let t := trace_of_ostrace et in
     forall t',
       is_trace z t' ->
       is_trace z0 (app_trace t t').
@@ -736,7 +749,7 @@ Section SpecsCorrect.
       (* The new itree 'consumed' the generated trace *)
       consume_trace z z' t /\
       (* t is the correct prefix *)
-      st'.(st_trace) = t ++ st.(st_trace) /\
+      st'.(io_log) = t ++ st.(io_log) /\
       (* The new trace is valid *)
       valid_trace st'.
   Proof.
